SDP v0.7

uexp/src/uexp/SDP_test.lean
@@ -17,7 +17,7 @@ end
 meta def inside_squash (e: expr) : tactic expr := 
     match e with 
     | `(usr.squash %%d) := tactic.to_expr ``(%%d)
-    | _ := tactic.fail "no squash to match"
+    | _ := do tactic.trace e, tactic.fail "no squash to match"
     end 
 
 meta def add_sqush (e: expr) : tactic expr :=
@@ -138,19 +138,70 @@ meta def first_in_squash (scope: tactic expr) : tactic expr := do
      | _ := tactic.fail "no squashed union in scope"
     end
 
+meta def is_one (e:expr) :bool :=
+match e with 
+| `(has_one.one usr) :=  true
+| _ := false
+end
+
+meta def unit_ueq_to_one (lp: list expr) : tactic (list expr) := do 
+    let f : expr → tactic expr := λ e,
+    match e with 
+    | `(%%a ≃ %%b) := if a = b then tactic.to_expr ``(has_one.one usr)
+                      else return e
+    | ex := return ex
+    end 
+    in do l ← monad.mapm f lp,
+        return $ list.filter (λ x, ¬ (is_one x)) l
+
+meta def prove_in_sig (n: nat) (solver: tactic unit ) : tactic unit := do
+    repeat_n n $ tactic.applyc `congr_arg >> tactic.funext,
+    solver
+
+/- simplification inside sigma 
+target: expr getter
+trans: transformation on AST
+solver: proof for transformation
+-/
+meta def simplify_in_sig (target: tactic expr) (trans: list expr → tactic (list expr)) (solver: tactic unit): tactic unit := do 
+    old ← target,
+    lsr ← return $ sigma_expr_to_sigma_repr old,
+    ⟨body, binders⟩ ← sigma_repr_to_closed_body_expr' lsr,
+    binders' ← return $ list.reverse binders,
+    let (exprs, names) := binders'.unzip,
+    lr ← product_to_repr body,
+    new_lr ← trans lr,
+    new_body ← repr_to_product new_lr,
+    abstracted ← return $ expr.abstract_locals new_body names, 
+    new ← sigma_repr_to_sigma_expr ⟨lsr.var_schemas, abstracted⟩, 
+    eq_lemma ← tactic.to_expr ``(%%old = %%new),
+    tactic.trace eq_lemma,
+    tactic.trace (list.length names),
+    ng_before ← list.length <$> tactic.get_goals,
+    lemma_name ← tactic.mk_fresh_name,
+    tactic.assert lemma_name eq_lemma,
+    tactic.trace (list.length names),
+    tactic.focus1 $ prove_in_sig (list.length names) solver, 
+    ng_after ← list.length <$> tactic.get_goals,
+    if ng_after > ng_before
+    then tactic.fail "simplify_inside_sig fail"
+    else (do
+    eq_lemma_name ← tactic.resolve_name lemma_name >>= tactic.to_expr,
+    tactic.rewrite_target eq_lemma_name,
+    tactic.clear eq_lemma_name)
+
+
 meta def unify_binder_i_j (i j: nat) : tactic unit := do
     add_lem i j, -- add lem of i-th and j-th binders
     split_lem, -- split plus inside sig
     distr_lem, -- distribute plus over sig
-    remove_dup_sigs (first_in_squash get_lhs),         -- remove dup sig on one side
-    
+    -- remove dup sig on one side
+    remove_dup_sigs (first_in_squash get_lhs),
+    -- simplify after remove_dup_sigs    
+     simplify_in_sig (first_in_squash get_lhs) unit_ueq_to_one `[repeat {rw eq_unit}, remove_all_unit],
     -- factorize
     -- reduce done
     return ()
-
-meta def try_me1 : tactic unit := do
-    ex ← first_in_squash get_lhs,
-    tactic.trace ex
 
 example {Γ s : Schema} (a : relation s) (g : Tuple Γ) (t : Tuple s):
 ∥(∑ (t₁ t₂ : Tuple s), denote_r a t₁ * (denote_r a t₂ * (t≃t₁)))∥ =
@@ -176,6 +227,14 @@ example {Γ s : Schema} {ty0 ty1 : datatype} (a : relation s) (c0 : Column ty0 s
                  ((denoteProj c1 t₁≃denoteProj c1 t₂) * (t≃(denoteProj c0 t₂, denoteProj c1 t₂))))))∥ =
     ∥(∑ (t_1 : Tuple s), denote_r a t_1 * (t≃(denoteProj c0 t_1, denoteProj c1 t_1)))∥ :=
 begin
+    add_lem 0 1,
+    split_lem,
+    distr_lem,
+    remove_dup_sigs $ first_in_squash get_lhs,
+    rw plus_comm,
+    remove_dup_sigs $ first_in_squash get_lhs,
+    rw plus_comm,
+    simplify_in_sig (first_in_squash get_lhs) unit_ueq_to_one `[repeat {rw eq_unit}, remove_all_unit],
     sorry, 
 end
 
@@ -191,5 +250,12 @@ example {Γ s1 s2 : Schema} (a : SQL Γ s1) (b : SQL Γ s2)
            ((denoteProj x t₁≃denoteProj x t₂) *
               (denoteSQL a g t₁ * (denoteSQL b g t₂_1 * (denoteSQL a g t₂ * (t≃denoteProj x t₁))))))∥ :=
 begin
+    apply ueq_symm,
+    add_lem 0 1,
+    split_lem,
+    distr_lem,
+    remove_dup_sigs $ first_in_squash get_lhs,
+    rw plus_comm,
+    remove_dup_sigs $ first_in_squash get_lhs,
     sorry,
 end
